simplifying premises

MultiScalarMul_Abstract.ec
@@ -1,7 +1,4 @@
-
-require import AllCore IntDiv CoreMap List Distr.
-
-require import AllCore Int IntDiv List StdOrder Bool.
+require import AllCore Int IntDiv List StdOrder Bool Distr.
 require import BitEncoding StdBigop Bigalg.
 (*---*) import Ring.IntID IntOrder BS2Int.
 (*---*) import Bigint BIA.
@@ -20,7 +17,6 @@ axiom l_pos : 0 < l.
 axiom T_pos : 0 < T.
 
 
-
 op perfect_table_pure  parg (varg : R) = 
  (fun (j i : int) =>  (i *** (parg j)) +++ - (2 ^ w - 1) *** varg).
 
@@ -32,8 +28,6 @@ axiom r_distr_full : is_full r_distr.
 axiom r_distr_uni : is_uniform r_distr.
 
 
-
-
 lemma r_distr_funi : is_funiform r_distr.
 proof. apply is_full_funiform.
 apply r_distr_full.
@@ -41,26 +35,27 @@ apply r_distr_uni.
 qed.
 
 
-
-
 module type OutCalls = {
   proc getU() : R
 }.
 
 
-op xdiff (x : R) (r : R) = xof x <> xof r.
+
 (* check the U candidate  *)
 op u_check (r : R) (P : int -> R) (s : int -> int -> int) : bool.
-
-(* check whether the table could be computed *)
-op table_check (P : int -> R) (r : R) : bool.
-
 
 op incompleteAddLoop (l : int) (argT : int -> int -> R)
   (args : int -> int -> int) (argic : int) (argcc : R) 
     = (iteri l (fun j (acc : bool * R) 
         => (acc.`1 /\ xdiff acc.`2 (argT j (args j argic)), 
              acc.`2 %%% argT j (args j argic))) (true, argcc)).
+
+
+op completeAddLoop (l : int) (argT : int -> int -> R)
+  (args : int -> int -> int) (argic : int) (argcc : R) 
+    = (iteri l (fun j (acc : bool * R) 
+        => (acc.`1 /\ xdiff acc.`2 (argT j (args j argic)), 
+             acc.`2  +++ argT j (args j argic))) (true, argcc)).
 
   
 op multiScalarMul (T l : int) (argT : int -> int -> R)
@@ -69,37 +64,21 @@ op multiScalarMul (T l : int) (argT : int -> int -> R)
         => let r = incompleteAddLoop l argT args i ((2 ^ argw) *** acc.`2) in 
          (acc.`1 /\ r.`1, r.`2)) (true, argu)).
 
+op multiScalarMul_Complete (T l : int) (argT : int -> int -> R)
+  (args : int -> int -> int) (argu : R) (argw : int)
+    = (iteri T (fun i (acc : bool * R) 
+        => let r = completeAddLoop l argT args i ((2 ^ argw) *** acc.`2) in 
+         (acc.`1 /\ r.`1, r.`2)) (true, argu)).
 
 
-op multiScalarMul_Simpl  (s : int -> int -> int) (P : int -> R) (ic jc : int)
+op multiScalarMul_Simpl  (s : int -> int -> int) (P : int -> R) (ic jc  : int)
   : R
  = iteri ic
      (fun i acc1 => acc1 +++ 
        iteri jc
          (fun j acc2 => 
-          acc2 +++ (2 ^ (w * (T - 1 - i)) * s j i) *** (P j)) idR
+          acc2 +++ (2 ^ (w * (ic - 1 - i)) * s j i) *** (P j)) idR
         ) idR.
-
-op gg (s : int -> int -> int) (P : int -> R) (i : int) (u : R) :  R 
-  = (multiScalarMul_Simpl s P i l) +++ l *** u.
-
-
-op hh (args : int -> int -> int)  (argP : int -> R)  (argic : int) (l : int) (u : R)
- =  2 ^ w *** gg args argP argic u +++  iteri l (fun j acc => acc +++ perfect_table_pure argP u j (args j argic)) idR.
-
-
-axiom muleqsimp i s u w P:
-   (multiScalarMul i l (perfect_table_pure P u) s (l *** u) w).`2
- = gg s P i u.
-
-
-axiom comeqsimp args argP  argic l r :
-  (iteri l
-   (fun (i1 : int) (acc0 : bool * R) =>
-      (acc0.`1 /\ xdiff acc0.`2 (perfect_table_pure argP r i1 (args i1 argic)),
-       acc0.`2 %%% perfect_table_pure argP r i1 (args i1 argic)))
-   (true, 2 ^ w *** gg args argP argic r)).`2
- = hh args argP argic l r .    
 
 
 
@@ -130,18 +109,20 @@ module SimpleComp = {
   }
 
   proc completeAddLoop(acc : R, table : int -> int-> R, ic : int, s : int -> int -> int) = {
-      var jc, aux, vahe;
+      var jc, aux, vahe, flag;
 
       aux <- witness;
+      flag <- true;
       jc <- 0;
       vahe <- acc;
       while (jc < l) {
         aux <- table jc (s jc ic);
+        flag <- flag /\ xdiff vahe aux;
         vahe <- vahe +++ aux;
 
         jc <- jc + 1;
       }
-      return vahe;
+      return (flag, vahe);
   }
 
 
@@ -164,24 +145,34 @@ module SimpleComp = {
   }
 
 
-  proc multiScalarMulMain_Perfect(P : int -> R, s : int -> int -> int, U : R) = {
+  proc multiScalarMulMain_Perfect_Helper(P : int -> R, s : int -> int -> int, U : R, Targ : int) = {
     var v, acc, aux, result : R;
     var table : int -> int -> R;
     var ic, jc, cnt : int;
+    var flagaux, flag : bool;
+    flagaux <- true;
+    flag <- true;
    
     v     <- (2 ^ w - 1) *** U;
-    table <- fun (j i : int) => (i *** (P j)) +++ - v;
+    table <- perfect_table_pure P U;
     acc   <- l *** U;
 
     ic <- 0;
-    while (ic < T) {
+    while (ic < Targ) {
       acc <@ doubleLoop(acc,w);
-      acc <@ completeAddLoop(acc, table, ic, s);
+      (flagaux, acc) <@ completeAddLoop(acc, table, ic, s);
+      flag <- flag && flagaux;
       ic <- ic + 1;
     }
     
-    result <- acc +++ (- (l *** U));
-    return result;
+    (* result <- acc +++ (- (l *** U)); *)
+    return (flag, acc);
+  }
+
+  proc multiScalarMulMain_Perfect(P : int -> R, s : int -> int -> int, U : R) = {
+     var result;
+     result <@ multiScalarMulMain_Perfect_Helper(P,s,U,T);
+     return  (result.`2 +++ (- (l *** U)));
   }
 
 
@@ -238,14 +229,12 @@ module SimpleComp = {
    (* check u *)
     flag   <- u_check u_cand P s;
     table  <- perfect_table_pure  P u_cand;
-    result <- multiScalarMul T l table s (l *** u_cand) w;
+    result <- multiScalarMul_Complete T l table s (l *** u_cand) w;
 
     return (flag /\ result.`1, result.`2 +++ (- (l *** u_cand)));
   }
 
-
 }.
-
 
 
 module MultiScalarMul(O : OutCalls) = {
@@ -253,17 +242,9 @@ module MultiScalarMul(O : OutCalls) = {
     var u_cand, result;
     u_cand <@ O.getU();
     result <@ SimpleComp.multiScalarMulMain_Opt_Corrected(P, s, u_cand);
-    return result;
+    return (result.`1, result.`2 +++ - l *** u_cand);
   }
 }.
-
-
-
-
-
-
-
-
 
 
 lemma doublewtimes_spec_ph argP argw :
@@ -284,39 +265,17 @@ move => z.
    smt(@Int).
 qed.
 
+
 lemma doublewtimes_spec argP argw :
  hoare [ SimpleComp.doubleLoop : arg = (argP, argw) /\
    0 <= argw  ==>  res = (2 ^ argw) *** argP  ].
 conseq (doublewtimes_spec_ph argP argw).   
 qed.   
 
-
-    
-
-lemma helper_specR_ph2 argcc argT argic args  : 
- phoare [ SimpleComp.completeAddLoop : arg = (argcc, argT, argic,  args) 
-     ==>  res = iteri l (fun j acc => acc +++ argT j (args j argic)) argcc ] = 1%r.
-proc.
-while (0 <= jc 
- /\ jc <= l 
- /\ (acc, table, ic,  s) = (argcc, argT, argic, args) 
- /\ vahe =    iteri jc (fun j acc => acc +++ argT j (args j argic)) acc) (l - jc).
-move => z.
-wp. skip. progress. smt(). smt(). rewrite iteriS. smt().
-   simplify.
-smt(op_assoc).
-smt().   
-   wp. skip. progress. smt(l_pos). 
-rewrite iteri0. auto.
-smt(op_id).
-smt().
-smt().
-qed.   
-
    
 lemma helper_specR_ph argcc argT argic args  : 
  phoare [ SimpleComp.completeAddLoop : arg = (argcc, argT, argic,  args) 
-     ==>  res = argcc +++  iteri l (fun j acc => acc +++ argT j (args j argic)) idR ] = 1%r.
+     ==>  res.`2 = argcc +++  iteri l (fun j acc => acc +++ argT j (args j argic)) idR ] = 1%r.
 proc.
 while (0 <= jc 
  /\ jc <= l 
@@ -345,23 +304,32 @@ auto.
 qed.    
 
 
+lemma doubleLoop_total  : 
+  phoare [ SimpleComp.doubleLoop : true ==>  true ] = 1%r.
+proc.
+while true (w - cnt). auto.
+smt().
+wp. auto. smt().
+qed.    
+
+
 lemma helper_specR argcc argT argic args  : 
  hoare [ SimpleComp.completeAddLoop : arg = (argcc, argT, argic,  args) 
-     ==>  res = argcc +++  iteri l (fun j acc => acc +++ argT j (args j argic)) idR ].
+     ==>  res.`2 = argcc +++  iteri l (fun j acc => acc +++ argT j (args j argic)) idR ].
 conseq (helper_specR_ph argcc argT argic args).   
 progress.
 qed.   
 
 
-lemma multiscalarR_spec argP args argU : 
- hoare [ SimpleComp.multiScalarMulMain_Perfect : 
-  arg = (argP, args, argU) 
-     ==>  res = (multiScalarMul_Simpl args argP T l)  ].
+lemma multiscalarR_helper_spec argP args argU  argT: 
+ hoare [ SimpleComp.multiScalarMulMain_Perfect_Helper : 
+  arg = (argP, args, argU, argT) 
+     ==>  res.`2 = (multiScalarMul_Simpl args argP argT l ) +++ l *** argU  ].
 proc. wp.
-while (0 <= ic
+while (0 <= ic /\ argT = Targ
  /\ (2 ^ w - 1) *** U = v
  /\ table = (fun (j i : int) =>  (i *** (P j)) +++ - v)
- /\ ic <= T
+ /\ ic <= argT
  /\ acc = ((iteri ic
             (fun i acc1 => acc1 +++
               (iteri l
@@ -371,7 +339,7 @@ wp.
 ecall (helper_specR acc table ic s). simplify.
 wp.
 ecall (doublewtimes_spec acc w). skip. progress. smt(w_pos).
-smt(). smt().
+smt(). smt(). rewrite H3.
    rewrite mul_plus_distr.
 rewrite iteriZ.           smt().
 simplify.
@@ -422,40 +390,43 @@ smt(). simplify.
 have ->: 2 ^ 0 = 1. smt(@Int).
 smt().
 wp. 
-skip. progress. smt(T_pos). 
+skip. progress. admit. 
 rewrite iteri0. auto. smt.
 rewrite /multiScalarMulInt.
-have -> : ic0 = T. smt().
-simplify.
-  have ->: iteri T
-  (fun (i : int) (acc1 : R) =>
-     acc1 +++
-     iteri l
-       (fun (j : int) (acc2 : R) =>
-          acc2 +++ 2 ^ (w * (T - 1 - i)) * s{hr} j i *** P{hr} j) idR) idR +++
-l *** U{hr} +++ - l *** U{hr}
-       = iteri T
-  (fun (i : int) (acc1 : R) =>
-     acc1 +++
-     iteri l
-       (fun (j : int) (acc2 : R) =>
-          acc2 +++ 2 ^ (w * (T - 1 - i)) * s{hr} j i *** P{hr} j) idR) idR +++
-  (l *** U{hr} +++ - l *** U{hr} ).
-smt(op_assoc).
-rewrite op_inv.
-  rewrite op_id.
-  rewrite /multiScalarMulR.
-auto.
+have -> : ic0 = Targ{hr}. smt().
+simplify. 
+rewrite /multiScalarMul_Simpl.
+(*   have ->: iteri T *)
+(*   (fun (i : int) (acc1 : R) => *)
+(*      acc1 +++ *)
+(*      iteri l *)
+(*        (fun (j : int) (acc2 : R) => *)
+(*           acc2 +++ 2 ^ (w * (T - 1 - i)) * s{hr} j i *** P{hr} j) idR) idR +++ *)
+(* l *** U{hr} +++ - l *** U{hr} *)
+(*        = iteri T *)
+(*   (fun (i : int) (acc1 : R) => *)
+(*      acc1 +++ *)
+(*      iteri l *)
+(*        (fun (j : int) (acc2 : R) => *)
+(*           acc2 +++ 2 ^ (w * (T - 1 - i)) * s{hr} j i *** P{hr} j) idR) idR +++ *)
+(*   (l *** U{hr} +++ - l *** U{hr} ). *)
+(* smt(op_assoc). *)
+(* rewrite op_inv. *)
+(*   rewrite op_id. *)
+(*   rewrite /multiScalarMulR. *)
+    reflexivity.
+(* auto. *)
 qed.
 
 
-lemma multiscalarR_spec_ph argP args argU : 
- phoare [ SimpleComp.multiScalarMulMain_Perfect : 
-  arg = (argP, args, argU) 
-     ==>  res = (multiScalarMul_Simpl args argP T l)  ] = 1%r.
+
+lemma multiscalarR_helper_spec_ph argP args argU argT : 
+ phoare [ SimpleComp.multiScalarMulMain_Perfect_Helper : 
+  arg = (argP, args, argU, argT) 
+     ==>  res.`2 = (multiScalarMul_Simpl args argP argT l) +++ l *** argU ] = 1%r.
 phoare split ! 1%r 0%r. auto.
    proc. wp.
-while true (T - ic). progress.
+while true (argT - ic). progress.
 wp.
 exists* acc, table, ic, s.
 elim*. move => accV tableV icV sV.
@@ -468,5 +439,171 @@ smt().
 wp. 
 skip. progress. smt().
 hoare. simplify.   
-apply multiscalarR_spec.
+apply multiscalarR_helper_spec.
+qed.
+
+
+lemma multiscalarR_spec_ph argP args argU  : 
+ phoare [ SimpleComp.multiScalarMulMain_Perfect : 
+  arg = (argP, args, argU) 
+     ==>  res = (multiScalarMul_Simpl args argP T l) ] = 1%r.
+proc.   
+call (multiscalarR_helper_spec_ph argP args argU T). auto.
+progress. smt.
+qed.
+
+
+lemma compelteAddLoop_ph argcc argT argic args  : 
+ phoare [ SimpleComp.completeAddLoop : arg = (argcc, argT, argic,  args) 
+     ==>  res = (completeAddLoop l argT args argic argcc) ] = 1%r.    
+proc.
+wp.   
+while (0 <= jc 
+ /\ jc <= l 
+ /\ (acc, table, ic,  s) = (argcc, argT, argic, args) 
+ /\ (flag, vahe) =  (iteri jc (fun j (acc : bool * R) => (acc.`1 /\ xdiff acc.`2 (argT j (args j argic)) , acc.`2 +++ argT j (args j argic))) (true, argcc))) (l - jc).
+move => z.
+wp. skip. progress. smt(). smt(). rewrite iteriS. smt().
+   simplify.
+   rewrite /xdiff. 
+pose xxx := (iteri jc{hr}
+     (fun (j : int) (acc0 : bool * R) =>
+        (acc0.`1 /\
+         xof acc0.`2 <> xof (table{hr} j (s{hr} j ic{hr})) && acc0.`2 <> idR,
+         acc0.`2 +++ table{hr} j (s{hr} j ic{hr}))) (true, acc{hr})).
+pose yyy := (iteri jc{hr}
+       (fun (j : int) (acc0 : R) => acc0 %%% table{hr} j (s{hr} j ic{hr}))
+       acc{hr}).     smt().
+ smt().
+(* smt(op_assoc). *)
+(* smt(). *)   
+   wp. skip. progress. smt(l_pos). 
+rewrite iteri0. auto. auto.
+(* rewrite iteri0. auto. auto. *)
+smt().   
+rewrite H2.
+         smt().
+qed.  
+
+
+lemma compelteAddLoop_h argcc argT argic args  : 
+ hoare [ SimpleComp.completeAddLoop : arg = (argcc, argT, argic,  args) 
+     ==>  res = (completeAddLoop l argT args argic argcc) ].
+conseq (compelteAddLoop_ph argcc argT argic args). qed.
+
+
+lemma multm_spec_h argP args argU  argT :
+ hoare [ SimpleComp.multiScalarMulMain_Perfect_Helper : arg = (argP, args, argU, argT)   
+  ==>  res = (multiScalarMul_Complete argT l (perfect_table_pure argP argU) args (l *** argU) w)   ] .
+proc. 
+while (argT = Targ /\
+  0 <= ic 
+  /\ ic <= argT
+  /\ (U, table, s) = (argU, (perfect_table_pure argP argU), args) 
+  /\ (flag, acc) = (multiScalarMul_Complete ic l ((perfect_table_pure argP argU)) args (l *** argU) w)
+ ) .
+wp.
+ecall (compelteAddLoop_h acc (perfect_table_pure argP argU) ic args).
+ecall (doublewtimes_spec acc w). 
+skip.
+progress. smt(w_pos).
+smt(). smt(). 
+rewrite /multiScalarMul_Complete. rewrite iteriS. smt(). smt(). 
+wp. skip. progress. admit.
+rewrite /multiScalarMul_Complete. rewrite iteri0.
+auto. auto. 
+have -> : Targ{hr} = ic0. smt(T_pos).
+auto.
+qed. 
+
+
+lemma multm_spec_ph argP args argU argT :
+ phoare [ SimpleComp.multiScalarMulMain_Perfect_Helper : arg = (argP, args, argU, argT)   
+  ==>  res = (multiScalarMul_Complete argT l (perfect_table_pure argP argU) args (l *** argU) w)   ] = 1%r .
+phoare split ! 1%r 0%r. auto.
+proc. while true (argT - ic). auto.
+call helper_specR_total.
+call doubleLoop_total.
+skip. smt().
+wp. skip. smt().
+hoare.
+proc*. ecall (multm_spec_h argP args argU argT).
+auto.
+qed.
+
+
+
+op gg (s : int -> int -> int) (P : int -> R) (i : int) (u : R) :  R 
+  = (multiScalarMul_Simpl s P i l) +++ l *** u.
+
+
+
+lemma oook argP (r : R) (argic : int)  args start : forall (n : int), 0 <= n =>
+   (iteri n
+   (fun (i1 : int) (acc0 : bool * R) =>
+      (acc0.`1 /\ xdiff acc0.`2 (perfect_table_pure argP r i1 (args i1 argic)),
+       acc0.`2 +++ perfect_table_pure argP r i1 (args i1 argic)))
+   (true, start)).`2
+    =    (iteri n
+   (fun (i1 : int) (acc0 : R) =>
+      (acc0 +++ perfect_table_pure argP r i1 (args i1 argic)))
+     start).
+apply intind. progress. 
+rewrite iteri0. auto.
+  rewrite iteri0. auto. auto.
+progress.
+rewrite iteriS. auto.
+  rewrite iteriS. auto.
+simplify.   rewrite H0. auto.
+qed.  
+  
+op hh (args : int -> int -> int)  (argP : int -> R)  (argic : int) (l : int) (u : R) =  2 ^ w *** gg args argP argic u +++  (iteri l
+   (fun (i1 : int) (acc0 : R) =>
+      (acc0 +++ perfect_table_pure argP u i1 (args i1 argic)))
+   idR).
+
+
+lemma comeqsimp args argP  argic l r :
+  (iteri l
+   (fun (i1 : int) (acc0 : bool * R) =>
+      (acc0.`1 /\ xdiff acc0.`2 (perfect_table_pure argP r i1 (args i1 argic)),
+       acc0.`2 +++ perfect_table_pure argP r i1 (args i1 argic)))
+   (true, 2 ^ w *** gg args argP argic r)).`2
+ = hh args argP argic l r .
+rewrite /hh. rewrite oook. 
+
+admit.
+
+rewrite  ( iteriZZZZZ (fun i1 => perfect_table_pure argP r i1 (args i1 argic))  (2 ^ w *** gg args argP argic r) l _ ). admit. smt.
+qed.
+
+
+lemma muleqsimp2 argT s u P :
+   gg s P argT u = (multiScalarMul_Complete argT l (perfect_table_pure P u) s (l *** u) w).`2 .
+rewrite /gg.
+case (multiScalarMul_Simpl s P argT l +++ l *** u = (multiScalarMul_Complete argT l (perfect_table_pure P u) s (l *** u) w).`2
+). 
+trivial.
+move => ineq.
+have : forall &m, 
+  Pr[ SimpleComp.multiScalarMulMain_Perfect_Helper(P,s, u,argT) @&m :
+     gg s P argT u = (multiScalarMul_Complete argT l (perfect_table_pure P u) s (l *** u) w).`2  ] = 1%r.
+     progress.
+     have ->: 1%r = Pr[ SimpleComp.multiScalarMulMain_Perfect_Helper(P,s, u,argT) @&m :
+         res.`2 = gg s P argT u ].
+    byphoare (_: arg = (P, s, u,argT) ==> _).
+    conseq (multiscalarR_helper_spec_ph P s u argT). auto. auto.
+    rewrite /gg. 
+    byequiv.
+    proc*.
+    ecall {2} (multm_spec_ph P s u argT).
+    ecall {1} (multiscalarR_helper_spec_ph P s u argT). skip. auto.
+    progress. rewrite  H0. auto. smt(). auto. auto. 
+   have : exists &m, true. smt().
+    elim. move => &h. auto.
+    move => _. rewrite /gg. move => p.
+    have : Pr[SimpleComp.multiScalarMulMain_Perfect_Helper(P, s, u, argT) @ &h :
+       false] = 1%r.
+     rewrite -  ineq. apply  (p &h).
+  smt(@Distr).
 qed.
